floyd/base.v
@@ -5,7 +5,6 @@ Require Export VST.msl.Extensionality.
 Require Export compcert.lib.Coqlib.
 Require Export VST.msl.Coqlib2 VST.veric.coqlib4 VST.floyd.coqlib3.
 Require Export VST.veric.juicy_extspec.
-(*Require Import VST.veric.NullExtension.*)
 Require Export VST.floyd.jmeq_lemmas.
 Require Export VST.floyd.find_nth_tactic.
 Require Export VST.floyd.val_lemmas.
@@ -127,7 +126,6 @@ Lemma sizeof_Tstruct: forall id a,
 Proof.
   intros. unfold sizeof.
   simpl. unfold get_co.
-  rewrite /lookup /composite_env_lookup /ptree_lookup.
   destruct (Maps.PTree.get id cenv_cs); auto.
 Qed.
 
@@ -136,7 +134,6 @@ Lemma sizeof_Tunion: forall id a,
 Proof.
   intros. unfold sizeof.
   simpl. unfold get_co.
-  rewrite /lookup /composite_env_lookup /ptree_lookup.
   destruct (Maps.PTree.get id cenv_cs); auto.
 Qed.
 
